Now it uses promising-lib/Language.t. Introduced a couple admits due to Coq weird behaviour.

src/promiseToImm/PromiseLTS.v
@@ -1,5 +1,5 @@
 From hahn Require Import Hahn.
-From Promising Require Import Language.
+Require Import PromisingLib.
 From Promising Require Import Event.
 Require Import Prog.
 Require Import ProgToExecution.
@@ -14,8 +14,8 @@ Definition lts_step (tid : thread_id) (pe : ProgramEvent.t) (s1 s2 : state) : Pr
     ⟪ISTEP: istep tid labels s1 s2⟫ /\
     ⟪LABS : lab_imm_promise labels pe⟫.
 
-Definition thread_lts (tid : thread_id) : Language.t :=
-  @Language.mk
+Definition thread_lts (tid : thread_id) : Language.t ProgramEvent.t :=
+  @Language.mk ProgramEvent.t
     (list Instr.t) state
     init
     is_terminal
