src/promiseToImm/PromisingLib.v
@@ -1,2 +1,1 @@
-From PromisingLib Require Export Basic DenseOrder Loc.
-From Promising Require Export Language.
+From PromisingLib Require Export Basic DenseOrder Loc Language.
