src/promiseToImm/SimState.v
@@ -1,5 +1,5 @@
 From hahn Require Import Hahn.
-From Promising Require Import Language.
+Require Import PromisingLib.
 
 Require Import Events Execution.
 Require Import ProgToExecution.
